

$$= \left| \frac{-3}{80} (e^6 - 1) \right| = \frac{3}{80} (e^6 - 1)$$

• Vector Space:

Let V be a set, whose elements are called vectors and F be a field, whose elements are called scalars. The set V is called vector space over the field F if $V(F)$ satisfy the following conditions:

• Vector Space:

1) Internal Composition
($A, +$)

$$A = \{ \alpha, \beta, \gamma, \theta, \delta \}$$

$$\alpha + \beta = \gamma$$

↓ Internal composition

2) External Composition

$$(B, +, \cdot)$$

$$B = \{ a, b, \dots \}$$

$$\alpha \cdot a = \beta$$

↓ External composition

1) $(V, +)$ is abelian group with respect to internal composition

2) $V(F)$ is closed under scalar multiplication with respect to external composition

$$\forall a \in F, \forall \alpha \in V$$

$$\Rightarrow a \cdot \alpha = \alpha \cdot a \in V$$

3) (V, \cdot) satisfy

a) $a \cdot \alpha \in V, \forall a \in F \text{ and } \forall \alpha \in V$

b) $a \cdot (\alpha + \beta) = a \cdot \alpha + a \cdot \beta \quad \forall a \in F \text{ and } \alpha, \beta \in V$

$$\begin{aligned} & c) a(bx) = (ab)x \} \forall 1, a, b \in F, x \in V \\ & d) 1 \cdot x = x \end{aligned}$$

$$Q) V = {}_R R^2 = \{(x, y) : x, y \in R\}$$

$F = R =$ Set of real numbers.

$$\begin{aligned} & (i) (V, +) \rightarrow \text{abelian group} \quad V = \{0, 1, 2, 3, 4\} \\ & \text{① Algebraic Structure} \\ & \text{② Monoid - identity} \quad 0 + 1 = 1 \\ & \text{③ Group - Inverse element} \quad 3 + 0 = 3 \end{aligned}$$

$$\begin{aligned} & (i) (V, +) \rightarrow \text{abelian group} \quad \xrightarrow{R} \quad \xrightarrow{R} \\ & (x, y) + (a, b) = (x + a, y + b) \end{aligned}$$

$$(0, 0) + (x, y) = (0 + x, 0 + y) = (x, y)$$

To check Inverse.

Identity

$$(x, y) + (-x, -y) = (0, 0)$$

$$\begin{aligned} & (ii) V \rightarrow (x, y) \in V, a \in F \\ & a \cdot (x, y) = (ax, ay) \in V \end{aligned}$$

$$4 \cdot (2, 5) = (4 \cdot 2, 4 \cdot 5) = (8, 20)$$

$$\begin{aligned} & (iii) \alpha, \beta \in V \quad a, b \in F \\ & (x_1, y_1) + (x_2, y_2) \quad a(\alpha + \beta) = a((x_1, y_1) + (x_2, y_2)) \end{aligned}$$

$$= (ax_1, ay_1) + (ax_2, ay_2)$$

$$= a(x_1 + x_2, y_1 + y_2) = a(x_1, y_1) + a(x_2, y_2)$$

$$= (ax_1 + ax_2, ay_1 + ay_2)$$

$$= (ax_1, ay_1) + (ax_2, ay_2) = a\alpha + a\beta$$

$$(a+b)\alpha = (a+b)(x_1, y_1)$$

$$= (a+b)x_1, (a+b)y_1$$

$$= (ax_1 + bx_1, ay_1 + by_1)$$

$$= (ax_1, ay_1) + (bx_1, by_1)$$

$$= a(x_1, y_1) + b(x_1, y_1)$$

$$= a\alpha + b\alpha$$

3 conditions satisfied.

• General Property of Vector Space :-

Let $V(F)$ be a vector space and $\bar{0}$ be a zero vector of V and 0 be the zero scalar of F then

Property:

$$1) a\bar{0} = \bar{0}, \forall a \in F$$

$$2) 0\alpha = \bar{0}, \forall \alpha \in V$$

$$3) a(-\alpha) = -(a\alpha), \forall a \in F, \forall \alpha \in V$$

$$4) (-a)\alpha = -(a\alpha), \forall a \in F, \forall \alpha \in V$$

$$5) a(\alpha - \beta) = a\alpha - a\beta, \forall a \in F, \forall \alpha, \beta \in V$$

$$① \quad a \alpha = \bar{0} \Rightarrow \alpha = \bar{0} \text{ or } a = 0, \forall a \in F, \forall \alpha \in V$$

• Proof :

$$① \quad a \bar{0} = \bar{0} \quad \forall a \in F$$

$$\bar{0} + \bar{0} = \bar{0}$$

$$a(\bar{0} + \bar{0}) = a\bar{0}$$

$$[a\bar{0} + \bar{0} = a\bar{0}]$$

$$a\bar{0} + a\bar{0} = a\bar{0} + \bar{0}$$

$$a\bar{0} = \bar{0}$$

$$② \quad 0 \alpha = \bar{0}$$

$$0 + 0 = 0$$

$$(0 + 0)\alpha = 0\alpha$$

$$0\alpha + 0\alpha = 0\alpha + \bar{0}$$

$$0\alpha = \bar{0}$$

$$\therefore 0\alpha + \bar{0} = 0\alpha$$

$$③ \quad \alpha + (-\alpha) = \bar{0}$$

$$a(\alpha + (-\alpha)) = a\bar{0}$$

$$a\alpha + a(-\alpha) = a\bar{0}$$

$$a\alpha + a(-\alpha) = \bar{0}$$

$$-(a\alpha) + a\alpha + a(-\alpha) = -(a\alpha) + \bar{0}$$

$$0 + a(-\alpha) = -(a\alpha)$$

$$a(-\alpha) = -(a\alpha)$$

$$④ \quad a + (-a) = 0$$

$$[a + (-a)]\alpha = 0\alpha$$

$$a\alpha + (-a)\alpha = 0\alpha$$

$$a\alpha + (-a)\alpha = \bar{0}$$

$$-(a\alpha) + a\alpha + (-a)\alpha = -(a\alpha) + \bar{0}$$

$$0 + (-a)\alpha = -(a\alpha)$$

$$[-a]\alpha = -(a\alpha)$$

$$\begin{aligned} a(x - \beta) &= a(x + (-\beta)) \\ &= ax + a(-\beta) \\ \boxed{a(x - \beta) &= ax - a\beta} \end{aligned}$$

by (3)

Q. a) Let $a \neq 0$
 $ax = \bar{0}$
 $a = 0, x = \bar{0}$

Now $ax = \bar{0}$
 $a^{-1}(ax) = a^{-1}\bar{0}$
 $(a^{-1}a)x = \bar{0}$
 $\boxed{x = \bar{0}}$

b) Let $x \neq \bar{0}$
 Start with contradiction $a \neq 0$
 $a^{-1} \in F, ax = \bar{0}$
 $a^{-1}(ax) = a^{-1}\bar{0}$
 $x = \bar{a}$

Our assumption is false.
 then

$$\boxed{a = 0}$$

• Pseudo Inverse :-

SVD

E.g. $C = \begin{bmatrix} 5 & 5 \\ -1 & 7 \end{bmatrix}$

$$\boxed{C = U \Sigma V^T}$$

$$\odot \quad C^T C = V \Sigma^T \Sigma V^T$$

$$\odot \quad C V = V \Sigma$$

$$\Rightarrow C^T C = \begin{bmatrix} 5 & -1 \\ 5 & 7 \end{bmatrix} \begin{bmatrix} 5 & 5 \\ -1 & 7 \end{bmatrix} = \begin{bmatrix} 26 & 18 \\ 18 & 74 \end{bmatrix}$$

$$\bullet \text{ Let } (C^T C - \lambda I) = 0$$

$$\begin{vmatrix} 26-\lambda & 18 \\ 18 & 74-\lambda \end{vmatrix} = 0$$

$$\lambda^2 - 100\lambda + 1600 = 0$$

$$\lambda = 20, 80$$

$$\bullet \lambda = 20$$

$$C C^T - 20 I = \begin{bmatrix} 6 & 18 \\ 18 & 54 \end{bmatrix}$$

$$V_1 = \begin{bmatrix} -\frac{3}{\sqrt{10}} \\ \frac{1}{\sqrt{10}} \end{bmatrix}$$

$$C C^T - 80 I = \begin{bmatrix} -54 & 18 \\ 18 & -6 \end{bmatrix}$$

$$V_2 = \begin{bmatrix} \frac{1}{\sqrt{10}} \\ \frac{3}{\sqrt{10}} \end{bmatrix}$$

$$\begin{pmatrix} 5 & 5 \\ -1 & 7 \end{pmatrix} \begin{pmatrix} -\frac{3}{\sqrt{10}} & \frac{1}{\sqrt{10}} \\ \frac{1}{\sqrt{10}} & \frac{3}{\sqrt{10}} \end{pmatrix} = \begin{pmatrix} -\sqrt{10} & 2\sqrt{10} \\ \sqrt{10} & 2\sqrt{10} \end{pmatrix}$$

$$C \quad V \quad = \begin{bmatrix} -\frac{1}{\sqrt{2}} & \frac{1}{\sqrt{2}} \\ \frac{1}{\sqrt{2}} & \frac{1}{\sqrt{2}} \end{bmatrix} \begin{bmatrix} \sqrt{5} & 0 \\ 0 & 4.5 \end{bmatrix}$$

$$= U \Sigma = \begin{bmatrix} 2\sqrt{5} & 0 \\ 0 & 4.5 \end{bmatrix}$$

$$U, V, \Sigma$$

$$A = U \Sigma V^T \rightarrow \text{Orthogonal matrix} \begin{pmatrix} V^T = V^{-1} \\ U^T = U^{-1} \end{pmatrix}$$

$$A^+ = (U \Sigma V^T)^{-1} = (V^{-1})^{-1} \Sigma^{-1} U^{-1}$$

Moore Inverse

$$A^+ = V \Sigma^{-1} U^T$$

$$\Sigma^{-1} = \begin{bmatrix} \frac{1}{\sigma_1} & & \\ & \frac{1}{\sigma_2} & \\ & & \frac{1}{\sigma_3} \end{bmatrix}$$

$$\sigma_1, \sigma_2, \sigma_3$$

Singular values $\sigma_1 = \sqrt{1}$

$$C = \begin{bmatrix} 5 & 5 \\ -1 & 7 \end{bmatrix}$$

$$U = \begin{bmatrix} -\frac{1}{\sqrt{2}} & \frac{1}{\sqrt{2}} \\ \frac{1}{\sqrt{2}} & \frac{1}{\sqrt{2}} \end{bmatrix}$$

$$V = \begin{bmatrix} -\frac{3}{\sqrt{10}} & \frac{1}{\sqrt{10}} \\ \frac{1}{\sqrt{10}} & \frac{3}{\sqrt{10}} \end{bmatrix}$$

$$V^T = \begin{bmatrix} -\frac{3}{\sqrt{10}} & \frac{1}{\sqrt{10}} \\ \frac{1}{\sqrt{10}} & \frac{3}{\sqrt{10}} \end{bmatrix}$$

$$\Sigma = \begin{bmatrix} 2\sqrt{5} & 0 \\ 0 & 4\sqrt{5} \end{bmatrix}$$

$$\Sigma^{-1} = \begin{bmatrix} \frac{1}{2\sqrt{5}} & 0 \\ 0 & \frac{1}{4\sqrt{5}} \end{bmatrix}$$

$$C = \begin{bmatrix} 5 & 5 \\ -1 & 7 \end{bmatrix}$$

$$\text{Find } C^T$$

$$C^T = V \Sigma^{-1} U^T$$

$$Q) A = \begin{bmatrix} 1 & 2 & 3 \\ 0 & 4 & 5 \end{bmatrix}$$

Find A^T ?

$$\text{Soln) } A^T A = \begin{bmatrix} & & \\ & & \\ & & \end{bmatrix}$$

$$\begin{aligned} &\rightarrow \lambda_1 \\ &\rightarrow \lambda_2 \\ &\rightarrow \lambda_3 \end{aligned}$$

$$\begin{aligned} \sigma_1 &= \sqrt{\lambda_1} \\ \sigma_2 &= \sqrt{\lambda_2} \\ \sigma_3 &= \sqrt{\lambda_3} \end{aligned}$$

$$\Sigma = \begin{bmatrix} \sigma_1 & & \\ & \sigma_2 & \\ & & \sigma_3 \end{bmatrix}$$

$$\lambda_1 = 54.1693$$

$$\lambda_2 = 0.8303$$

$$\lambda_3 = 0$$

$$X = \begin{bmatrix} 1 \\ 3 \\ 2 \end{bmatrix} = \frac{1}{\sqrt{1^2 + 3^2 + 2^2}} = \begin{bmatrix} \frac{1}{\sqrt{14}} \\ \frac{3}{\sqrt{14}} \\ \frac{2}{\sqrt{14}} \end{bmatrix} \quad \text{Higher Unit vectors}$$

$$X_1 = \begin{bmatrix} -0.675 \\ -0.6067 \\ -0.7921 \end{bmatrix}, \quad X_2 = \begin{bmatrix} -0.9521 \\ 0.2764 \\ -0.1306 \end{bmatrix}$$

$$V = \begin{bmatrix} -0.675 & -0.9521 & -0.2981 \\ -0.6067 & 0.2764 & -0.7454 \\ -0.7921 & -0.1306 & 0.5963 \end{bmatrix} \quad \text{can ask this}$$

$$CV = U \Sigma$$

$$CV =$$

$$U =$$

$$U = \begin{bmatrix} -0.4969 & -0.8678 \\ -0.8678 & 0.4969 \end{bmatrix}$$

$$\Sigma = \begin{bmatrix} 7.36 & 0 & 0 \\ 0 & 0.914 & 0 \\ 0 & 0 & 0 \end{bmatrix}$$

can ask this

$$A^+ =$$

can ask this

Q1) Show that the set $W = \{(a, b, 0) : a, b \in F\}$ is a subspace of $V_3(F)$.

Soln) Let $\alpha = (a_1, b_1, 0)$, $\beta = (a_2, b_2, 0)$

i.e. $\alpha, \beta \in W$, and $a, b \in F$

$$\begin{aligned} \text{Now } a\alpha + b\beta &= a(a_1, b_1, 0) + b(a_2, b_2, 0) \\ &= (aa_1, ab_1, 0) + (ba_2, bb_2, 0) \\ &= (aa_1 + ba_2, ab_1 + bb_2, 0) \end{aligned}$$

Since, $\forall a_1, b_1, a_2, b_2, a, b \in F$
 \rightarrow scalars

$$\Rightarrow aa_1 + ba_2 \in F \quad ab_1 + bb_2 \in F$$

$$\Rightarrow a\alpha + b\beta = (aa_1 + ba_2, ab_1 + bb_2) \in W$$

$\Rightarrow W$ is a subspace of $V(F)$.

(2) $W = \left\{ \begin{bmatrix} a & b \\ -b & a \end{bmatrix} : a, b \in F \right\}$ is a subspace of $M_2(F)$

(Soln) Let $\alpha = \begin{bmatrix} a_1 & b_1 \\ -b_1 & a_1 \end{bmatrix}$, $\beta = \begin{bmatrix} a_2 & b_2 \\ -b_2 & a_2 \end{bmatrix}$

i.e. $\alpha, \beta \in W$, and, $a, b \in F$

$$\text{Now } a\alpha + b\beta = a \begin{bmatrix} a_1 & b_1 \\ -b_1 & a_1 \end{bmatrix} + b \begin{bmatrix} a_2 & b_2 \\ -b_2 & a_2 \end{bmatrix}$$

$$= \begin{bmatrix} aa_1 & ab_1 \\ -ab_1 & aa_1 \end{bmatrix} + \begin{bmatrix} ba_2 & bb_2 \\ -bb_2 & ba_2 \end{bmatrix}$$

$$= \begin{bmatrix} aa_1 + ba_2 & ab_1 + bb_2 \\ -ab_1 - bb_2 & aa_1 + ba_2 \end{bmatrix}$$

Since, $\forall a_1, b_1, a_2, b_2, a, b \in F$
 \rightarrow scalars.

$$\Rightarrow aa_1 + ba_2, \dots \in F$$

$$\Rightarrow a\alpha + b\beta = \begin{bmatrix} \dots \\ \dots \end{bmatrix} \in W.$$

$\Rightarrow W$ is a subspace of $V(F)$.